{
 "cells": [
  {
   "cell_type": "markdown",
   "metadata": {},
   "source": [
    "We will consider more families of differential equations in this lesson."
   ]
  },
  {
   "cell_type": "markdown",
   "metadata": {},
   "source": [
    "## More families of ODEs\n",
    "### Autonomous\n",
    "$\\frac{\\operatorname{d} x}{\\operatorname{d} t} = f(x)$, as the derivative only depends on $x$.\n",
    "### Non-autonomous\n",
    "$\\frac{\\operatorname{d} x}{\\operatorname{d} t} = f(x, t)$, which are usually very difficult to solve. Some of them however, are solvable.\n",
    "\n",
    "### Separable\n",
    "\n",
    "$\\frac{\\operatorname{d} x}{\\operatorname{d} t} = f(x) g(t)$. Then following the pattern of linear differentiation, we can separate the ODE as $$\n",
    "\\begin{array}{l}\n",
    "\\frac{\\operatorname{d} x}{f(x)} &= g(t) \\operatorname{d} t \\\\\n",
    "\\int \\frac{1}{f(x)} \\operatorname{d} x &= \\int g(t) \\operatorname{d} t \\\\\n",
    "\\end{array}\n",
    "$$"
   ]
  },
  {
   "cell_type": "markdown",
   "metadata": {},
   "source": [
    "### Example: Drag force\n",
    "\n",
    "Assume a drag force proportional to velocity. What is the velocity of the body at time $t$?\n",
    "\n",
    "Let $m$ be the mass, and $g$ be the gravitational constant, then the gravitational force the body is subject to is $m g$.\n",
    "\n",
    "Meanwhile, the drag force is $- \\kappa v$, where $\\kappa$ is a constant. Then we have $$\n",
    "m \\frac{\\operatorname{d} v}{\\operatorname{d} t} = m g - \\kappa v\n",
    "$$. This ODE is *autonomous* and *separable*. By doing a little factoring we have $$\n",
    "\\begin{array}{l}\n",
    "m \\frac{\\operatorname{d} v}{\\operatorname{d} t} &= m g - \\kappa v \\\\\n",
    "m \\frac{\\operatorname{d} v}{\\operatorname{d} t} &= \\kappa (\\frac{m g}{\\kappa} - v) \\\\\n",
    "\\frac{\\operatorname{d} v}{\\frac{m g}{\\kappa} - v} &= \\frac{\\kappa}{m} \\operatorname{d} t \\\\\n",
    "\\frac{\\operatorname{d} v}{v - \\frac{m g}{\\kappa}} &= - \\frac{\\kappa}{m} \\operatorname{d} t \\\\\n",
    "\\int \\frac{1}{v - \\frac{m g}{\\kappa}} \\operatorname{d} v &= \\int - \\frac{\\kappa}{m} \\operatorname{d} t \\\\\n",
    "\\ln(v - \\frac{m g}{\\kappa}) &= - \\frac{\\kappa}{m} t + C \\\\\n",
    "v - \\frac{m g}{\\kappa} &= e^{- \\frac{\\kappa}{m} t + C} \\\\\n",
    "&= C e^{- \\frac{\\kappa}{m} t} \\\\\n",
    "v &= C e^{- \\frac{\\kappa}{m} t} + \\frac{m g}{\\kappa}\n",
    "\\end{array}\n",
    "$$. What if $t$ goes to infinity? $$\n",
    "\\begin{equation}\n",
    "\\begin{aligned}\n",
    "\\lim_{t \\to \\infty} v(t) &= \\lim_{t \\to \\infty} (C e^{- \\frac{\\kappa}{m} t} + \\frac{m g}{\\kappa}) \\\\\n",
    "&= 0 + \\frac{m g}{\\kappa} \\\\\n",
    "&= \\frac{m g}{\\kappa}\n",
    "\\end{aligned}\n",
    "\\end{equation}\n",
    "$$. This is called the *terminal velocity*."
   ]
  },
  {
   "cell_type": "markdown",
   "metadata": {},
   "source": [
    "### Example: Torricelli's law\n",
    "\n",
    "This model is for the fluid leaking from the tank.\n",
    "\n",
    "![](torricellis_law.png)\n",
    "\n",
    "$$\n",
    "\\begin{equation}\n",
    "\\begin{aligned}\n",
    "\\frac{\\operatorname{d} h}{\\operatorname{d} t} &= - \\frac{\\kappa}{A} \\sqrt{h} \\\\\n",
    "&= - \\frac{\\kappa}{\\pi h^2} \\sqrt{h} & \\text{As the tank is a cone which area $A$ is proportional to $h$} \\\\\n",
    "&= - \\frac{\\kappa}{\\pi} h^{-\\frac{3}{2}} \\\\\n",
    "h^{\\frac{3}{2}} \\operatorname{d} h &=  - \\frac{\\kappa}{\\pi} \\operatorname{d} t \\\\\n",
    "\\int h^{\\frac{3}{2}} \\operatorname{d} h &= \\int - \\frac{\\kappa}{\\pi} \\operatorname{d} t \\\\\n",
    "\\frac{2}{5} h^{\\frac{5}{2}} &= - \\frac{\\kappa}{\\pi} t + C \\\\\n",
    "h &= (- \\frac{5 \\kappa}{2 \\pi} t + C)^{\\frac{2}{5}}\n",
    "\\end{aligned}\n",
    "\\end{equation}\n",
    "$$. What that implies is $h$ approaches to $0$ very rapidly: $O((t_{end} - t)^{\\frac{2}{5}})$."
   ]
  },
  {
   "cell_type": "markdown",
   "metadata": {},
   "source": [
    "### Linear *non-autonomous* ODE'S\n",
    "\n",
    "$$\n",
    "\\frac{\\operatorname{d} x}{\\operatorname{d} t} = A(t) x + B(t)\n",
    "$$. We mean *linear* as if we suppress $t$ dependent, we have $$\n",
    "\\frac{\\operatorname{d} x}{\\operatorname{d} t} = A x + B\n",
    "$$\n",
    "\n",
    "For example $$\n",
    "\\frac{\\operatorname{d} x}{\\operatorname{d} t} = t x + \\frac{1}{2} t^2\n",
    "$$. How do we solve such kind of ODE's? The method we are going to introduce is called **integrating factor**, which we denote by $\\operatorname{I}$. $$\n",
    "\\begin{array}{l}\n",
    "\\operatorname{I}(\\frac{\\operatorname{d} x}{\\operatorname{d} t} &= A x + B) \\\\\n",
    "\\operatorname{I}(\\frac{\\operatorname{d} x}{\\operatorname{d} t} - A x &= B) \\\\\n",
    "\\operatorname{I} \\frac{\\operatorname{d} x}{\\operatorname{d} t} - A \\operatorname{I} x &= \\operatorname{I} B\n",
    "\\end{array}\n",
    "$$. Let's pause for a moment. If we can transform the above equation into $$\n",
    "\\operatorname{I} \\frac{\\operatorname{d} x}{\\operatorname{d} t} + \\frac{\\operatorname{d} \\operatorname{I}}{\\operatorname{d} t} x = \\operatorname{I} B\n",
    "$$, then from the product rule, we will have $$\n",
    "\\operatorname{d} (\\operatorname{I} x) = \\operatorname{I} B\n",
    "$$. So what needs to be true to have the above equation holds? We will need $$\n",
    "\\begin{array}{l}\n",
    "- A \\operatorname{I} x &= \\frac{\\operatorname{d} \\operatorname{I}}{\\operatorname{d} t} x \\\\\n",
    "\\frac{\\operatorname{d} \\operatorname{I}}{\\operatorname{d} t} &= - A \\operatorname{I}\n",
    "\\end{array}\n",
    "$$. And this equation is *separable*, which means $$\n",
    "\\begin{array}{l}\n",
    "\\frac{\\operatorname{d} \\operatorname{I}}{\\operatorname{d} t} &= - A \\operatorname{I} \\\\\n",
    "\\frac{\\operatorname{d} \\operatorname{I}}{\\operatorname{I}} &= - A \\operatorname{d} t \\\\\n",
    "\\int (\\frac{\\operatorname{d} \\operatorname{I}}{\\operatorname{I}} &= - A \\operatorname{d} t) \\\\\n",
    "\\int \\frac{1}{\\operatorname{I}} \\operatorname{d} \\operatorname{I} &= - \\int A \\operatorname{d} t \\\\\n",
    "\\ln(\\operatorname{I}) &= - \\int A\\\\\n",
    "\\operatorname{I} &= e^{- \\int A }\n",
    "\\end{array}\n",
    "$$. So we choose $I$ to be $$\n",
    "\\operatorname{I} = e^{- \\int A}\n",
    "$$, then we will have $$\n",
    "\\begin{array}{l}\n",
    "\\operatorname{d} (\\operatorname{I} x) &= \\operatorname{I} B \\\\\n",
    "\\int (\\operatorname{d} (\\operatorname{I} x) &= \\operatorname{I} B) \\\\\n",
    "\\int \\operatorname{d} (\\operatorname{I} x) &= \\int \\operatorname{I} B \\\\\n",
    "\\operatorname{x} &= \\frac{1}{\\operatorname{I}} \\int \\operatorname{I} B \\\\\n",
    "&= e^{\\int A} (\\int B e^{- \\int A}) \\\\\n",
    "&= e^{\\int A(t) \\operatorname{d} t} (\\int B(t) e^{- \\int A(t)} \\operatorname{d} t) \\\\\n",
    "\\end{array}\n",
    "$$"
   ]
  },
  {
   "cell_type": "markdown",
   "metadata": {},
   "source": [
    "#### Example: Mixing\n",
    "\n",
    "A $1000$ gallon tank is $90\\%$ full.\n",
    "\n",
    "An additive is injected into the tank at rate $10$ gallon/minute.\n",
    "\n",
    "The mixture is well-stripped and drained at rate of $5$ gallon/minute.\n",
    "\n",
    "What is the concentration of the additive when the tank is full?\n",
    "\n",
    "Let\n",
    "- $V(t)$ be the volume at time $t$.\n",
    "- $Q(t)$ be the quantity of the additive at time $t$.\n",
    "- $C(t)$ be the concentration at time $t$, that $C(t) = \\frac{Q(t)}{V(t)}$.\n",
    "\n",
    "Then we have $$\n",
    "V(t) = 900 + (10 - 5) t\n",
    "$$, and we then know the tank will be full in 20 minutes.\n",
    "\n",
    "We also know that $$\n",
    "\\begin{array}{l}\n",
    "\\frac{\\operatorname{d}}{\\operatorname{d} t} Q = 10 - 5 C \\\\\n",
    "&= 10 - 5 \\frac{Q}{V} \\\\\n",
    "&= 10 - \\frac{Q}{180 + t} \\\\\n",
    "\\frac{\\operatorname{d}}{\\operatorname{d} t} Q + \\frac{Q}{180 + t} &= 10\n",
    "\\end{array}\n",
    "$$. That means the integrating factor $\\operatorname{I}$ is $$\n",
    "\\begin{array}{l}\n",
    "\\operatorname{I} &= e^{\\int \\frac{1}{180 + t} \\operatorname{d} t} \\\\\n",
    "&= e^{\\ln(180 + t)} \\\\\n",
    "&= 180 + t\n",
    "\\end{array}\n",
    "$$. Then we can multiply the original ODE by the integrating factor $\\operatorname{I}$: $$\n",
    "\\begin{array}{l}\n",
    "\\frac{\\operatorname{d}}{\\operatorname{d} t} Q &= 10 - \\frac{Q}{180 + t} \\\\\n",
    "\\operatorname{I} \\frac{\\operatorname{d}}{\\operatorname{d} t} Q + \\operatorname{I} \\frac{Q}{180 + t} &= \\operatorname{I} \\cdot 10 \\\\\n",
    "(180 + t) \\frac{\\operatorname{d}}{\\operatorname{d} t} Q + (180 + t) \\frac{Q}{180 + t} &= (180 + t) \\cdot 10 \\\\\n",
    "(180 + t) \\frac{\\operatorname{d}}{\\operatorname{d} t} Q + Q &= (180 + t) \\cdot 10 \\\\\n",
    "\\operatorname{d} ((180 + t) Q) &= 10 (180 + t) \\\\\n",
    "\\int \\operatorname{d} ((180 + t) Q) &= \\int 10 (180 + t) \\operatorname{d} t \\\\\n",
    "(180 + t) Q &= 1800 t + 5 t^2 + C \\\\\n",
    "(180 + t) Q &= 1800 t + 5 t^2 + 0 &\\text{as the initial quantity of the additive is $0$} \\\\\n",
    "Q &= \\frac{1800 t + 5 t^2}{180 + t} \\\\\n",
    "Q(20) &= \\frac{1800 t + 5 t^2}{180 + t}|_{t = 20} \\\\\n",
    "&= 190 \\\\\n",
    "C(20) &= \\frac{V(20)}{Q(20)} \\\\\n",
    "&= \\frac{190}{1000} \\\\\n",
    "&= 19 \\%\n",
    "\\end{array}\n",
    "$$"
   ]
  },
  {
   "cell_type": "code",
   "execution_count": null,
   "metadata": {},
   "outputs": [],
   "source": []
  }
 ],
 "metadata": {
  "kernelspec": {
   "display_name": "Python 3",
   "language": "python",
   "name": "python3"
  },
  "language_info": {
   "codemirror_mode": {
    "name": "ipython",
    "version": 3
   },
   "file_extension": ".py",
   "mimetype": "text/x-python",
   "name": "python",
   "nbconvert_exporter": "python",
   "pygments_lexer": "ipython3",
   "version": "3.7.0"
  }
 },
 "nbformat": 4,
 "nbformat_minor": 2
}
